\documentclass{article}
\usepackage[utf8x]{inputenc}
\usepackage[T1, T2A]{fontenc}
\usepackage[russian]{babel}
\usepackage{amsmath}
\usepackage{amssymb}
\setlength\parindent{0pt}
\usepackage[parfill]{parskip}
\pagenumbering{gobble}

\begin{document}
Заметим, что 
$$x_{k+1} - x_k = \frac{x_k + kx_{k-1}}{k+1} - x_k = \frac{k}{k+1} (x_{k-1} - x_k) = $$
$$ = \frac{-k}{k+1} (x_k - x_{k-1}) = \frac{(-1)^k}{k+1} (x_1 - x_0) = \frac{(-1)^k}{k+1}.$$
Поскольку
$$\lim_{k \to \infty} (x_{k+1} - x_k) \to 0,$$
ряд сходится.

Найдем теперь члены ряда:
$$x_n = \sum_{k=1}^n (x_k - x_{k-1}) = \sum_{k=1}^n \frac{(-1)^{k+1}}{k}.$$

Поскольку 
$$\ln(t + 1) = \sum_{k=1}^\infty \frac{(-1)^{k+1}t^k}{k},$$
находим, что
$$\lim_{n \to \infty} x_n = \ln 2.$$
\end{document}
